TM/Code/WriteValue.v
@@ -1,0 +1,43 @@
+Require Import CodeTM.
+Require Import TM.Basic.WriteString.
+Require Import Basic.Mono.
+
+
+Lemma WriteString_L_right (sig : finType) (str : list sig) t :
+  right (WriteString_Fun L t str) = rev str ++ right t.
+Proof.
+  revert t. induction str; intros; cbn in *.
+  - reflexivity.
+  - rewrite IHstr. simpl_tape. rewrite <- app_assoc. reflexivity.
+Qed.
+
+Arguments WriteString_Fun : simpl never.
+
+Section WriteValue.
+
+  Variable (sig: finType) (X: Type) (cX: codable sig X).
+
+  Definition WriteValue (x:X) : { M : mTM sig^+ 1 & states M -> unit } :=
+    WriteString L (inl STOP :: rev (encode x));; Write (inl START) tt.
+
+  Definition WriteValue_Rel (x : X) : Rel (tapes sig^+ 1) (unit * tapes sig^+ 1) :=
+    Mk_R_p (ignoreParam (fun tin tout => isRight tin -> tout ≃ x)).
+
+
+  Lemma WriteValue_Sem (x : X) :
+    WriteValue x ⊨c(5 + 3 * length (cX x)) WriteValue_Rel x.
+  Proof.
+    eapply RealiseIn_monotone.
+    { unfold WriteValue. repeat TM_Correct. eapply WriteString_Sem. }
+    { cbn. rewrite rev_length, map_length. apply Nat.eq_le_incl. omega. }
+    {
+      intros tin ((), tout) H. intros HRight.
+      TMSimp; clear_trivial_eqs.
+      repeat econstructor. f_equal. rewrite WriteString_L_right. cbn.
+      rewrite <- app_assoc.
+      rewrite rev_involutive.
+      rewrite isRight_right; auto.
+    }
+  Qed.
+
+End WriteValue.
